extended invariant example (send a message and set a new state) + needed lemmas for that

examples/invariants/DY.Example.Invariants.fst
@@ -3,6 +3,7 @@ module DY.Example.Invariants
 open Comparse
 open DY.Core
 module L = DY.Lib
+module List = FStar.List.Tot.Base
 
 /// Experimenting with the new state invariants for sessions and full states
 
@@ -14,6 +15,17 @@ type p_state =
 
 instance parseable_serializeable_bytes_p_state: parseable_serializeable bytes p_state
  = mk_parseable_serializeable ps_p_state
+
+
+type message =
+  | M: alice:principal -> message
+
+%splice [ps_message] (gen_parser (`message))
+%splice [ps_message_is_well_formed] (gen_is_well_formed_lemma (`message))
+
+instance parseable_serializeable_bytes_message: parseable_serializeable bytes message
+ = mk_parseable_serializeable ps_message
+
 
 // let max_nat (x:nat) (y:nat) : nat = max x y
 
@@ -53,6 +65,7 @@ let next prin sid =
   match parse p_state curr_state with
   | None -> return None
   | Some (S idn c) -> (
+         send_msg (serialize message (M prin));*
          set_state prin sid (serialize p_state (S idn (c+1)));*
          return (Some ())
   )
@@ -62,21 +75,73 @@ let p_cinvs = {
  preds = default_crypto_predicates default_crypto_usages
 }
 
+
+let rec map_rev_list f xs =
+  match xs with
+  | Nil -> Nil
+  | Snoc init x -> Snoc (map_rev_list f init) (f x)
+
+let rec all_some xs =
+  match xs with
+  | Nil -> true
+  | Snoc init x -> Some? x && (all_some init)
+
+val all_some_lemma:
+  #a : eqtype ->
+  xs:rev_list (option a) ->
+  Lemma 
+    (requires all_some #a xs
+    )
+    (ensures
+      has_type xs (rev_list (x:option a{Some? x}))
+    )
+let all_some_lemma #a xs = admit()
+  
+let parse_session session_b =
+    let parsed_session = map_rev_list (parse #_ p_state #parseable_serializeable_bytes_p_state) session_b in
+    if all_some parsed_session
+      then ( 
+        all_some_lemma parsed_session;
+        Some (map_rev_list (fun s -> Some?.v s) parsed_session )
+      )
+      else None
+
+
+let parse_full_state (fst_b: full_state_raw ) : list (state_id * option (rev_list p_state))=
+  FStar.List.Tot.Base.map (fun (sid, sess) -> (sid, parse_session sess)) fst_b
+
 let p_state_pred: state_predicate p_cinvs = {
     pred = (fun tr p sid cont -> is_knowable_by #p_cinvs (principal_state_label p sid) tr cont)
   ; session_pred = (fun tr sess prin sid cont -> 
       match sess with
-      | Nil -> True
+      | Nil -> True // session is empty -> delegate to (single state) pred
       | Snoc init last -> (
           match (parse p_state last, parse p_state cont) with
           | (None,_) -> False
           | (_,None) -> False
-          | (Some (S idn ctr), Some (S idn' ctr') ) -> ctr < ctr' 
+          | (Some (S idn ctr), Some (S idn' ctr') ) -> ctr < ctr' /\ idn = idn'
       )
     )
-  ; full_state_pred = (fun tr fst p sid cont -> True)
+  ; full_state_pred = (fun tr fst_b p sid cont -> 
+      let full_st = parse_full_state fst_b in
+      True
+      // forall (i:nat{i < List.length full_st}). 
+      //   match List.index full_st i with 
+      //   | (_, None) -> True // or False ?
+      //   | (_, Some Nil) -> True
+      //   | (sid_i, Some (Snoc init_i last_i)) ->
+      //     if sid_i = sid 
+      //       then True
+      //       else begin
+      //         match parse p_state cont with
+      //         | None -> False
+      //         | Some (S idn' ctr') -> last_i.idn <> idn'
+      //       end
+      
+  )
   ; pred_later = (fun t1 t2 p sid cont -> ())
   ; pred_knowable = (fun tr p sid cont -> ())
+  ; session_pred_grows = (fun tr1 tr2 sess p sid cont -> ())
 }
 
 instance protocol_invariants_p: protocol_invariants = {
@@ -87,7 +152,34 @@ instance protocol_invariants_p: protocol_invariants = {
   }
 }
 
+val send_msg_no_state:
+  msg:bytes -> tr:trace ->
+  Lemma 
+    ( let (_, tr_out) = send_msg msg tr in 
+      forall p sid. no_set_state_entry_for p sid (tr_out `suffix_after` tr)
+    )
+  [SMTPat (send_msg msg tr)]
+let send_msg_no_state msg tr = 
+  reveal_opaque (`%send_msg) send_msg;
+  reveal_opaque (`%get_state) get_state
 
+
+// let prefix_including_event ev tr =
+//   Snoc (prefix_before_event ev tr) ev
+
+// let rec prefix_including_event_is_prefix the_ev tr : 
+//   Lemma (prefix_including_event the_ev tr <$ tr) [SMTPat (prefix_including_event the_ev tr)] =
+//   reveal_opaque (`%grows) grows;
+//   norm_spec [zeta; delta_only [`%prefix]] (prefix);
+//   match tr with
+//   | Nil -> ()
+//   | Snoc init ev ->
+//          if ev = the_ev
+//            then ()
+//            else prefix_including_event_is_prefix the_ev init
+
+// TODO: this proof is slow and unstable
+#push-options "--z3rlimit 25"
 val next_invariant: tr:trace -> p:principal -> sid:state_id ->
   Lemma 
     (requires trace_invariant tr)
@@ -102,7 +194,38 @@ let next_invariant tr p sid =
   | (Some st_b, _) -> (
       match parse p_state st_b with
       | None -> ()
-      | Some (S idn c) -> (
-          serialize_wf_lemma p_state (is_knowable_by (principal_label p) tr) (S idn (c+1))
-    )
-    )
+      | Some (S idn c) -> (          
+          let msg = M p in
+          let msg_b = serialize message msg in
+          let (_, tr_after_msg) = send_msg msg_b tr in
+
+          let next_state = S idn (c+1) in
+          let next_state_b = serialize p_state next_state in
+          let (_,tr_after_next_state) = set_state p sid next_state_b tr_after_msg in
+          
+
+          //assume(trace_invariant tr_after_next_state)
+
+          serialize_wf_lemma message (is_publishable tr) msg;
+          // assert(is_publishable tr msg_b);
+          // assert(trace_event_invariant tr (MsgSent msg_b ));
+
+          serialize_wf_lemma p_state (is_knowable_by (principal_state_label p sid) tr_after_msg) next_state;
+          // assert(state_pred tr_after_msg p sid next_state_b);
+          
+          //let session_after_msg = get_session p sid tr_after_msg in          
+          let session_before_msg = get_session p sid tr in                  
+          // assert(tr <$ tr_after_msg);
+          assert(no_set_state_entry_for p sid (tr_after_msg `suffix_after` tr));
+          assert(session_pred_opt tr session_before_msg p sid next_state_b);
+          session_pred_later tr tr_after_msg p sid next_state_b;
+          // assert(global_state_pred tr_after_msg p sid next_state_b);
+          // assert(trace_event_invariant tr_after_msg (SetState p sid next_state_b))
+
+           
+//           ; let full_st_b_tr = get_full_state p tr in
+//             let full_st_b_pref = get_full_state p (prefix_before_event (SetState p sid (serialize p_state (S idn c))) tr) in
+//           assume(full_st_b_pref = full_st_b_tr)
+// //          assume(full_state_pred_opt tr full_st_b p sid st_b)
+    ()
+    ))
